%---------------------------------------------------
% Exponential (& Logarithmic) Functions
%---------------------------------------------------
\chapter[Exponential Functions]{Exponential \& Logarithmic \\Functions}
%\section{placeholder}
We defined $a^{x}$ where $a >0$ in chapter 1, however $x$ was restricted to rational numbers. We now want to explore $a^{x}$ where $a >0$ and $x$ is any real number. 

We can show that values exist simply by pressing buttons on the calculator or drawing
a graph using Desmos, however an intuitive understanding can be obtained by considering appropriate values. 

Consider $2^{\pi }$. We know $\pi  =3.141592654 \ldots $. $2^{\pi }$ should be between $2^{3}$\ and $2^{4}$. That is between $8$ and $16$. We can evaluate 

\qquad \qquad \qquad \qquad \qquad \qquad \qquad \qquad
\begin{tabular}[c]{ll}$2^{3.1}$  & $8.5741877$  \\
	$2^{3.14}$  & $8.815240927$  \\
	$2^{3.141}$  & $8.821353305$  \\
	$2^{3.1415}$  & $8.824411082$  \\
	$2^{3.14159}$  & $8.824961595$  \\
	$2^{3.141592}$  & $8.824973829$  \\
	$2^{3.1415926}$  & $8.824977499$  \\
	$2^{3.14159265}$  & $8.824977805$  \\
	$2^{3.141592654}$  & $8.82497783$
\end{tabular}

We could continue this process. If
we enter $2^{\pi }$ on the calculator the answer obtained is
\begin{equation*}2^{\pi } =8.824977827
\end{equation*}

The graph of $y =2^{x}$, $ \forall x \in \mathbb{R}$ is shown. 
\includegraphics[width=3.7758in, height=2.1378in,]{L4SZ282M}

Recall $y =f (x)$ is a function and $y =f ( -x)$ is the same function with every $x$ replaced with $ -x$, i.e. $y =f ( -x)$ is the reflection of $y =f (x)$ in the $y$-axis. 

If $y =2^{x}$ then $y =2^{ -x}$ is the reflection of $y =2^{x}$ in the $y$-axis. But $y =2^{ -x} =\left (2^{ -1}\right )^{x} =\genfrac{(}{)}{}{}{1}{2}^{x}$. 

\textbf{Graphing Exercise} Use Desmos to verify that $y =2^{-x}$ and $y =\frac{1}{2}^x$ are equivalent. 

\subsection*{The Exponential Function $f(x)=a^x$}
Let $y =a^{x}$ where $a >0$ 

\begin{center}
\begin{tabular}{lcl}
	\toprule
	When $0 <a <1$  & $y =a^{x}$ looks like  &    
	\includegraphics[ width=1.9086in, height=1.0853in,]{L4SZ282O}
	\\
	\midrule
	When $a =1$  & $y =a^{x} =1^{x} =1$ looks like  &    
	\includegraphics[ width=1.9095in, height=1.1234in,]{L4SZ282P}
	\\
	\midrule
	When $a >1$  & $y =a^{x}$ looks like  &    
\includegraphics[ width=1.9372in, height=1.0741in,]{L4SZ282Q}
	\\
	\bottomrule
\end{tabular}
\end{center}

$f (x) =a^{x}$ is called an \emph{exponential} function. $a$ is called the \emph{base} of the exponential function. The domain
is $\mathbb{R}$. the range is $\left (0 ,\infty \right )$. The $x$-axis is an asymptote. 

\textbf{Example 1} Find the equation of the exponential function that passes through $\left (0 ,1\right )$ and $\left (3 ,125\right )$. 

\textbf{Solution} An exponential function that passes through $\left (0 ,1\right )$ is of the form $f (x) =a^{x}$. As $f (3) =125$ we substitute $x =3$ and get
\begin{align*}a^{3} &  = 125 \\
a &  = \sqrt[{3}]{125} =5\\
\therefore f(x)&=5^x \text{ satisfies the conditions.}
\end{align*}

\subsection*{Transformations of Exponential Functions}
Recall the transformations we have met so far 

\begin{center}
\begin{tabular}{ll}Vertical stretch of $a$  & $y =f (x) \leadsto y =a f (x)$  \\
	Horizontal stretch of $\frac{1}{b}$  & $y =f (x) \leadsto y =f (b x)$  \\
	Vertical shift of $c$ $\uparrow $  & $y =f (x) \leadsto y =f (x) +c$  \\
	Horizontal shift of $d$ $ \longrightarrow $  & $y =f (x) \leadsto y =f (x -d)$  \\
	Reflection in $x$-axis  & $y =f (x) \leadsto y = -f (x)$  \\
	Reflection in $y$-axis  & $y =f (x) \leadsto y =f ( -x)$
\end{tabular}
\end{center}
Each of these transformations can be applied to an exponential
function. 

\textbf{Graphing Exercise} Given $y =2^{x}$ apply the following transformations. Draw a sketch showing where the graph crosses the $y$-axis, its shape, its asymptote and one other point it passes through. 

\columnseprule =0.4pt
\begin {multicols}{2}
\begin{enumerate}
	\item Horizontal shift of $ +2\vspace{+2.000000cm}$ 
	
	\item Vertical shift of $ -3\vspace{+2.000000cm}$ 
	
	\item Horizontal stretch of $2\vspace{+2.000000cm}$ 
	
	\item Vertical stretch of $4\vspace{+2.000000cm}$ 
	
	\item Horizontal stretch of $\frac{1}{3}\vspace{+2.000000cm}$ 
	
	\item Vertical stretch of $\frac{1}{2}\vspace{+2.000000cm}$ 
	
	\item Reflection in the x-axis\vspace{2cm}
	
	
	\item Reflection in the y-axis\vspace{2cm} 
	
	\item (Challenge) Reflection in $y = -1\vspace{+2.000000cm}$ 
	
	\item (Challenge) Reflection in $x =1\vspace{+4.000000cm}$ \end{enumerate}

\end {multicols}
\medskip\medskip\medskip\medskip

%---------------------------------------------------
% the natural exponential function e^x
%---------------------------------------------------
%\section{\texorpdfstring{$e^x$}{}}
\section[$e^x$]{The Natural Exponential Function}
The \emph{natural exponential function} has wide application in mathematics engineering. It arises naturally and crops up in applications such as finance, population, radioactivity, charge on a capacitor, and more. We have defined $f (x) =a^x$ and there is a particular value of $a$ that we denote by the letter $e$. It is an irrational number (like $\pi $, $\sqrt{2}$ etc.) and has a button on your calculator. To 10 decimal places it is
\[e \approx 2.7182818285\dots\]
The natural exponential function $f (x) =e^x$ is often simply referred to as \textit{the} exponential function. 

Compound interest can demonstrate an example of  how the value above is found. Imagine a bank that pays 100\% interest on your money. Given an initial deposit of \$1, at the end of year you will receive \$1 in interest payment and have a total of \$2. Compounded interest allows this to happen at intervals smaller than 1 year. If the interest is compounded twice per year, then after 6 months, you will receive 50\% interest and have \$1.50. In the second half of the year you now have an additional \$0.50 available to earn the second half interest. Now, $\$1.50\times50\%=\$0.75$, so at the end of the year you have \$1.50+\$0.75=\$2.25.

Lets say the interest is compounded monthly, then after 1 month you will receive $\frac{1}{12}\times 100\%=8.33\%$ interest for \$1+\$0.0833=\$1.0833. The second month will earn the same rate (8.33\%) on \$1.0833, for a total of \$1.1736. After 12 months, your dollar will now be worth $\$1.00\times\left(1+\frac{1}{12}\right)^{12}=\$2.6130$. 
\begin{center}
\begin{tabular}{cll}
	\toprule
	compounding periods&interest (\$)&total (\$)\\
	\midrule
	1 (yearly)&1.00&2.00\\
	2&1.25&2.25\\
	3&1.3704 &2.3704\\
	4 (quarterly)& 1.4414 & 2.4414 \\
	5& 1.48832 & 2.48832 \\
	6& 1.521626&2.521626\\\midrule
	12 (monthly)& 1.613035&2.613035 \\\midrule
	52 (weekly)&1.692597 &2.692597\\\midrule
	365 (daily)&1.714567 &2.714567\\\midrule
	continuous& 1.718282&\textbf{2.718282$\dots$}\\
	\bottomrule
\end{tabular}
\end{center}

As a function this is plotted below:

This comes up again in the following chapters.


%---------------------------------------------------
% Logarithmic Functions
%---------------------------------------------------
\section{Logarithmic Functions}
The \emph{logarithmic function} is the inverse of the function $f (x) =a^{x}$. Recall the inverse of a function is the reflection of the function in the line $y =x$. Mathematically this is equivalent to swapping the $x$ and the y in $y =a^{x}$. So $x =a^{y}$ is the inverse of $y =a^{x}$. We have another notation for the inverse of a function, which is a little more complicated.
\ let $y =f (x)$ be a function of $x$ then $y =f^{ -1} (x)$ is the inverse of this function. Sometimes the inverse of the function is also a function.
\ For example the inverse of $y =x^{2}$ is $x =y^{2}$. $y =x^{2}$ is a function (vertical line test always applies), whereas $x =y^{2}$ is not a function (vertical line test is broken). 


\includegraphics[ width=3.032in, height=2.4275in,]{L4SZ2832}



The inverse of $y =10^{x}$ is $x =10^{y}$. $y =10^{x}$ is a function (vertical line test always applies) and so is $x =10^{y}$. 


\includegraphics[ width=2.3419in, height=2.4267in,]{L4SZ2833}



Another useful fact to remember about inverses concerns the domain and range. The \emph{domain}
of $f$ is the \emph{range} of $f^{ -1}$ and the \emph{range} of $f$ is the \emph{domain} of $f^{ -1}$. 

We have a notation for $x =a^{y}$ it is $y =\log _{a} x$:
\begin{tcolorbox}
\[y =\log _{a} x \Leftrightarrow x =a^y
\]
\end{tcolorbox}


In $x =a^{y}$ substitute $y =\log _{a} x$ and we get $x =a^{\log _{a} x}$. This means that given a base of $a$ the power (or exponent) to which $a$ must be raised to get $x$ is $\log _{a} x$. 

Problems involving logarithms will often require us to switch back and forth between $y =\log _{a} x$ and $x =a^{y}$, however it is also helpful if you can remember to substitute for $y$ and write $x =a^{\log _{a} x}$ so that you can say ``the logarithm is the power". 

\textbf{Example 1}
\begin{description}
	\item [(a)] $\log _{10} 100 =2$ because $10^{2} =100$ 
	
	\item [(b)] $\log _{3} 81 =4$ because $3^{4} =81$ 
	
	\item [(c)] $\log _{10} 0.01 = -2$ because $10^{ -2} =0.01$ \end{description}

\subsection*{The graph of $y =\log _{a} x$}
The exponential function $y =a^{x}$ where $a >0$ is now known and its domain is $\mathbb{R}$ and its range is the positive real numbers. We often
write $\mathbb{R}^{ +}$ instead of $\left (0 ,\infty \right )$. 

The graph of $f (x) =a^{x}$ can be reflected in the line $y =x$ and the result is $f^{ -1} (x) =\log _{a} x$. 

\textbf{Graphing Exercise} On the same set of axes draw:
\begin{tasks}(4)
	\task $y =10^{x}$ 
	\task $y =\log _{10} x$ 
	\task $y =x$ 
	\task $x =10^{y}$ 
\end{tasks}

Make a comment about each statement below. 
\begin{tasks}
	\task[1.] Check the graphs in (a), (b) and (c) are you confident that $y =\log _{10} x$ is the reflection of $y =10^{x}$ in the line $y =x$?
	\task[2.] When you enter $x =10^{y}$ describe what takes place.
	\end{tasks}

\textbf{Graphing Exercise Solution} Using \desmos we can see the different plots. Plots (b) and (d) are equivalent, so are on top of each other.\\
\begin{center}\vspace{-1cm}
\includegraphics[width=14cm]{logGraph1}\\
\end{center}

\textbf{Graphing Exercise} On the same set of axes draw:
\begin{tasks}(4)
	\task $y =\log _{2} x$ 
	\task $y =\log _{3} x$ 
	\task $y =\log _{4} x$ 
	\task $y =\log _{10} x$ \end{tasks}
\textbf{Graphing Exercise Solution} Using \desmos we can see the relationship between the different bases in the log equation:\\
\begin{center}\vspace{-1cm}\includegraphics[width=14cm]{logGraph2}\end{center}
Notice the point that is common to all curves and the behaviour of the family of curves for $x >1$ and for $0 <x <1$. 

\textbf{Property 1}: A property of logarithms is $\log _{a} 1 =0$ and this can be seen on the graphs where every graph goes through $\left (1 ,0\right )$. 

The pattern you observe as the base gets bigger might not be evident for values of the base between $0$ and $1$. On the same set of axes draw the following: 

\begin{tasks}(4)
	\task $y =\log _{\frac{1}{2}} x$ 
\task $y =\log _{\frac{1}{3}} x$ 
	\task $y =\log _{\frac{1}{4}} x$ 
	\task $y =\log _{\frac{1}{5}} x$ \end{tasks}
\begin{center}\vspace{-0.5cm}\includegraphics[width=14cm]{logGraph3}\end{center}
To say the pattern is the same you have to be careful to describe the base. Explain how changing the base gives the same pattern as for (a) to (d).

\textbf{Property 2:} A second property of logarithms is $\log _{a} a =1$. That is $a^{1} =a$ or the power to which you have to raise $a$ to get $a$ is $1$. On your curves above locate a point on each curve that shows this. You
should in each case be looking for the point $\left (a ,1\right )$. 

\textbf{Property 3:} A third property
of logarithms is $\log _{a} a^{x} =x$. This useful property must be understood if logarithm problems are to be mastered.
\ You should understand what $\log _{a} a^{x}$ is saying. $a$ is the base so $\log _{a} a^{x} =x$ says ``The power to which $a$ must be raised to get $a^{x}$ is $x$." 

\subsection*{Common Logarithms}
When the base is $10$ we write $y =\log _{10} x =\log  x$. If you see no base you assume it is base $10$. $y =\log  x$ is called the \emph{common} logarithm of $x$. Desmos and other programs with mathematics incorporated recognise "$\log $" as "logarithm to the base $10$". The $\log $ key on the calculator gives the common logarithm of any positive number.
\begin{tcolorbox}
\begin{equation*}y =\log  x \Leftrightarrow 10^{y} =x
\end{equation*}
\end{tcolorbox}


\subsection*{Natural Logarithms}
When the base is $e$ we write $y =\log _{e} x =\ln  x$. If you see $\ln  x$ you assume it is $\log _{e} x$. $y =\ln  x$ is called the \emph{natural} logarithm of $x$. Desmos and other programs with mathematics incorporated recognise "$\ln $" as "logarithm to the base $e$". The $\ln $ key on the calculator gives the natural logarithm of any positive number.
\begin{tcolorbox}\begin{equation*}y =\ln  x \Leftrightarrow e^{y} =x
\end{equation*}\end{tcolorbox}

\textbf{Graphing Exercise}
Use Desmos to sketch the following. Describe in words how each curve is related to $y =\ln  x$. 

\begin{tasks}(3)
	\task $y =\ln  x$ 
\task  $y =\ln  ( -x)$ 
\task  $y = -\ln  x$ 
	\task  $y =\ln  (x -1)$ 
	\task  $y =\ln  (x) -1$ 
	\task $y =\ln  ( -1 -x)$ \end{tasks}


\subsection*{The Laws of Logarithms}
\begin{tcolorbox}
\begin{tasks}[label-width={10em}]
	\task[Law 1:] $\qquad\log _{a} \left (X Y\right ) =\log _{a} X +\log _{a} Y$ 	
	\task[Law 2:] $\qquad\log _{a} \left(\frac{X}{Y}\right) =\log _{a} X -\log _{a} Y$ 	
	\task[Law 3:] $\qquad\log _{a} X^{c} =c \log _{a} X$ 
\end{tasks}
\end{tcolorbox}

It is a useful exercise to prove these laws as the proofs show the
connection between the laws for exponents and the laws for logarithms. 

\textbf{Proof of Law 1} \\\relax Let
$\log _{a} X =u$ so $a^{u} =X$ \\\relax and $\log _{a} Y =v$ so $a^{v} =Y$ \\\relax $X Y =a^{u} a^{v} =a^{u +v}$ \\\relax Take logarithms of both sides to the base $a$ \\\relax $\log _{a} X Y =\log _{a} a^{u +v} =u +v$ {\scriptsize (property 3)} $ =\log _{a} X +\log _{a} Y$ 

\textbf{Proof of Law 2} \\\relax $\frac{X}{Y} =\frac{a^{u}}{a^{v}} =a^{u -v}$ \\\relax Take logarithms of both sides to the base $a$ \\\relax $\log _{a} \frac{X}{Y} =\log _{a} a^{u -v} =u -v$ {\scriptsize (property 3)} $ =\log _{a} X -\log _{a} Y$ 

\textbf{Proof of Law 3} \\\relax $X^{c} =\left (a^{u}\right )^{c} =a^{u c} =a^{c u}$ \\\relax Take logarithms of both sides to the base $a$ \\\relax $\log _{a} X^{c} =\log _{a} a^{c u} =c u$ {\scriptsize (property 3)} $ =c \log _{a} X$ 

\textbf{Example 1}
Expand using the logarithm laws 
\begin{description}
	\item [(a)] $\log  \sqrt{3} =\log  3^{\frac{1}{2}} =\frac{1}{2} \log  3$ 
	
	\item [(b)] $\ln  \genfrac{(}{)}{}{}{a \sqrt{b}}{\sqrt[{3}]{c}} =\ln  \left (a b^{\frac{1}{2}} c^{ -\frac{1}{3}}\right ) =\ln  a +\ln  b^{\frac{1}{2}} +\ln  c^{ -\frac{1}{3}} =\ln  a +\frac{1}{2} \ln  b -\frac{1}{3} \ln  c$ \end{description}

\textbf{Example 2}
Evaluate
\begin{description}
	\item [(a)] $\log _{2} 112 -\log _{2} 7 =\log _{2} \frac{112}{7} =\log _{2} 16 =\log _{2} 2^{4} =4 \log _{2} 2 =4$ 
	
	\item [(b)] $\log _{2} 8^{23} =\log _{2} \left (2^{3}\right )^{23} =\log _{2} \left (2^{69}\right ) =69 \log _{2} 2 =69$ 
	
	\item [(c)] $\log  \sqrt{0.001} =\log  \left (0.001\right )^{\frac{1}{2}} =\frac{1}{2} \log  0.001 =\frac{1}{2} \log  10^{ -3} =\frac{1}{2} \times  -3 = -\frac{3}{2} = -1\frac{1}{2}$ 
	
	\item [(d)] $e^{2 \ln  4} =\left (e^{\ln  4}\right )^{2} =4^{2} =16\text{\quad \quad }($Let $\ln  4 =x$ then $e^{x} =4$ so $e^{\ln  x} =4)$ \end{description}

\textbf{Example 3}
Rewrite as a single logarithm term using the logarithm laws 
\begin{description}
	\item [(a)] $\log  12 +\frac{1}{2} \log  5 -\log  3 =\log  \frac{12 \sqrt{5}}{3} =\log  4 \sqrt{5}$ 
	
	\item [(b)] $\log _{3} \left (x^{2} -1\right ) -\log _{3} \left (x -1\right ) =\log _{3} \frac{x^{2} -1}{x -1} =\log _{3} \frac{\left (x +1\right ) \left (x -1\right )}{x -1} =\log _{3} \left (x +1\right )$ \end{description}



%---------------------------------------------------
% Exponential and Logarithmic Equations
%---------------------------------------------------
\section{Exponential and Logarithmic Equations}
The types of problems we meet in this section will be able to be rearranged so that they look like
\begin{equation*}a^{f (x)} =b
\end{equation*}

Where $a$ and $b$ are real numbers, $x$ is the unknown variable we are trying to find and $f (x)$ is an expression in $x$. The technique we will use will be the same for every problem we solve. 


\begin{description}
	\item [Step 1] Our first step is to inspect the problem to see if the unknown
	variable is in the exponent. 
	
	\item [Step 2] Now that we have
	established that we are solving an exponential equation we rearrange it until it is in the form $a^{f (x)} =b$ 
	
	\item [Step 3] Take the logarithm
	of both sides. In most practical situations we either take logarithms to the base $10$ or logarithms to the base $e$. there are three situations 
	
	\item [Case
	1] The problem has reduced to $10^{f (x)} =b$. Take logarithms to the base $10$. 
	
	\item [Case 2] The problem has
	reduced to $e^{f (x)} =b$. Take logarithms to the base $e$. 
	
	\item [Case 3] The problem has
	reduced to $a^{f (x)} =b$ where $a$ is neither $10$ nor $e$. You can take logarithms to the base $10$ or $e$ as you wish, either is correct. 
	
	\item [Step 4]
	Solve the equation you obtain. \end{description}

\textbf{Example 1} Solve $3^{x} =5$. This is an example of case $3$ above.\\ 
\textbf{Solution} 
\begin{tasks}[label-width={5em}](2)
\task[Method 1] \\Take logarithms to the base $10$\\
\begin{align*}\log  3^{x} &  = \log  5 \\
x \log  3 &  = \log  5 \\
x &  = \frac{\log  5}{\log  3} \\
&  \approx 1.464973521 \approx 1.46\text{(2 dp)}\end{align*}
\task[Method 2] \\Take logarithms to the base $e$\\
\begin{align*}\ln  3^{x} &  = \ln  5 \\
x \ln  3 &  = \ln  5 \\
x &  = \frac{\ln  5}{\ln  3} \\
&  \approx 1.464973521 \approx 1.46\text{(2 dp)}\end{align*}
\end{tasks}
This shows it is immaterial whether you take logarithms to base $10$ or logarithms to base $e$. 
\begin{tasks}[label-width={6em}](2)
\task[Example 2]
Solve $3^{2 x +1} =5$\\
\textbf{Solution} Take logarithms to the base 10:
\begin{align*}\log  3^{2 x +1} &  = \log  5 \\
\left (2 x +1\right ) \log  3 &  = \log  5 \\
2 x +1 &  = \frac{\log  5}{\log  3} \\
2 x &  = \frac{\log  5}{\log  3} -1 \\
x &  = \frac{1}{2} \left (\frac{\log  5}{\log  3} -1\right ) \\
&  \approx 0.23248676 \approx 0.23\text{(2 dp)}\end{align*}

\task[Example 3]
Solve $4 \left (1 +10^{5 x}\right ) =9$\\
\textbf{Solution} This must first be rearranged:
\begin{align*}1 +10^{5 x} &  = \frac{9}{4} =2.25 \\
10^{5 x} &  = 2.25 -1 =1.25 \\
\text{}{\scriptsize 10}\text{}\log  10^{5 x} &  = \log  1.25 \\
5 x &  = \log  1.25 \\
x &  = \frac{1}{5} \log  1.25 \\
&  \approx 0.019382002 \approx 0.019\text{(3 dp)}\end{align*}
\end{tasks}

\textbf{Example 4} Solve $\frac{10}{1 +e^{ -x}} =3$.
\begin{align*}1 +e^{ -x} &  = \frac{10}{3} \\
e^{ -x} &  = \frac{10}{3} -1 \\
&  = \frac{10 -3}{3} =\frac{7}{3} \\
-x &  = \ln  7 -\ln  3 \\
x &  \approx  -0.85\text{(2 dp)}\end{align*}


\subsection*{Solving Logarithmic Equations}
Whereas exponential equations have the unknown variable in an exponent, logarithmic equations are equations containing the logarithm of an unknown variable. 

\begin{description}
	\item [Step 1] You recognise you are dealing with a logarithmic equation
	by inspecting the problem to see if you have a logarithm of a term containing the unknown variable. 
	
	\item [Step	2] Rearrange the equation until it is in the form
	\begin{equation*}\log _{a} \left (\text{term containing unknown}\right ) =b
	\end{equation*} where $b$ is a number. 
	
	\item [Step 3] Take	``antilogarithms ". That is if $\log _{a} X =b$ then $a^{b} =X$ 
	
	\item [Step 4] Solve the equation.
	($a$ and $b$ are known and $X$ is an expression containing the unknown variable.) \end{description}

\textbf{Example 1} Solve $\ln  x =5$ .\\
\textbf{Solution} Take antilogarithms with base $e$:
\begin{align*}e^{5} &  = x \\
x &  \approx 148.4131591 \approx 148.4\text{(1 dp)}\end{align*}

\textbf{Example 2} Solve $5 +4 \log  \left (5 x\right ) =17$.\\
\textbf{Solution} Isolate the log and solve:
\begin{align*}4 \log  \left (5 x\right ) &  = 17 -5 =12 \\
\log  5 x &  = 3 \\
\text{}10^{3} &  = 5 x \\
x &  = \frac{1000}{5} =200\end{align*}

Check:\ Substitute $x =200$
\begin{align*}\text{LHS} &  = 5 +4 \log  \left (5 \times 200\right ) \\
&  = 5 +4 \log  1000 =5 +4 \log  10^{3} \\
&  = 5 +4 \times 3 =5 +12 =17 =\text{RHS}\end{align*}

\begin{tasks}[label-width={6em}](2)
	\task[Example 3]\\
Solve $\log  x +\log  \left (x -1\right ) =\log  4 x$
\begin{align*}\log  x +\log  \left (x -1\right ) -\log  4 x &  = 0 \\
\log  \frac{x \left (x -1\right )}{4 x} &  = 0 \\
\log  \frac{1}{4} \left (x -1\right ) &  = 0 \\
\text{}10^{0} &  = \frac{1}{4} \left (x -1\right ) =1 \\
x -1 &  = 4 \\
x &  = 5\end{align*}

Check:
\begin{align*}\text{LHS} &  = \log  5 +\log  4 =\log  \left (5 \times 4\right ) =\log  20 \\
\text{RHS} &  = \log  4 \times 5 =\log  20 =\text{LHS}\end{align*}

\task[Example 4] The velocity of a sky diver $t$ \\seconds after jumping is given by
\begin{equation*}v \left (t\right ) =80 \left (1 -e^{ -0.2 t}\right )
\end{equation*}

After how many seconds is the velocity $70$ $\mbox{ft}$/$\mbox{s}$?
\begin{align*}70 &  = 80 \left (1 -e^{ -0.2 t}\right ) \\
\frac{70}{80} &  = 1 -e^{ -0.2 t} \\
e^{ -0.2 t} &  = 1 -\frac{70}{80} \\
&  = 1 -\frac{7}{8} =\frac{1}{8} =0.125 \\
\text{} -0.2 t &  = \ln  0.125 \\
t &  = \frac{\ln  0.125}{ -0.2} \approx 10.39\text{}\mbox{s}\end{align*}
\end{tasks}

%---------------------------------------------------
% Exponential Modelling
%---------------------------------------------------
\section{Exponential Modelling}
The natural exponential function, $e^x$, is used in a variety of situations where there is exponential growth or decay. 

\textbf{Example} The exponential function can be used to model the way populations grow and diseases spread. The following
example is about the spread of an infectious disease in a small city whose population is $10,000$. After $t$ days the number of people who have caught the disease is modelled by the function
\begin{equation*}f (t) =\frac{10000}{5 +2495 e^{ -0.84 t}}
\end{equation*}


\begin{tasks}
	\task How many people had the disease initially? 
	\textbf{Solution} \textit{Initially} in this sense means right at the beginning, or when the clock is still at zero. Substitute $t=0$ into the function:
	\[f(0)=\frac{10000}{5+2495e^0}=\frac{10000}{2500}=4\text{ people}\]
	\task How many people have the disease after 1 day?
	\textbf{Solution} Substitute $t=1$ into the function:
	\[f(1)=\frac{10000}{5+2495e^{-0.84}}=\frac{10000}{5+2495(0.4317)}=\frac{10000}{1082.1}\approx 9.24;\text{ 9 people}\]
	\task How many people have the disease after 5 days? 
	\textbf{Solution} Following from part (b), find $f(5)$:\\
	\[f(5)=\frac{10000}{5+2495e^{-0.84(5)}}=\frac{10000}{42.41}\approx 235.77;\text{ 236 people}\]
	
	\task Use desmos to graph the function and describe its behaviour. \\
	%\includegraphics[width=\textwidth]{modelling1}
	\includegraphics[width=\textwidth]{logGraph1}
\end{tasks}

The graph has distinctive characteristics. It starts at a particular nonzero value (when $t =0$) and increases slowly at first then more rapidly. It slows down after a time and levels off because the exponential function in the denominator $ \leadsto 0$ when $t \leadsto \infty $. Graphs with these characteristics are called logistic curves. The particular model is called a logistic growth model. 

%---------------------------------------------------
% Chapter Exercises in a separate file
%---------------------------------------------------
\section{Chapter Exercises}
\subimport{}{expExercises}

% END ----------------------------------------------